Prove adapted print program

dimsum_examples/print.v
@@ -17,6 +17,15 @@ Definition print_args (z : Z) (args : list Z) : Prop :=
 Definition print_asm : gmap Z asm_instr :=
   deep_to_asm_instrs print_addr [
       Amov "R8" __NR_PRINT;
+      (* Aadd "R0" "R0" 0; *)
+      Asyscall;
+      Aret
+    ].
+
+Definition print_asm' : gmap Z asm_instr :=
+  deep_to_asm_instrs print_addr [
+      Amov "R8" __NR_PRINT;
+      Aadd "R0" "R0" 0;
       Asyscall;
       Aret
     ].
@@ -26,6 +35,24 @@ Definition print_spec : spec asm_event unit void :=
     '(rs, mem) ← TReceive (λ '(rs, mem), (Incoming, EAJump rs mem));
     TAssume (rs !!! "PC" = print_addr);;
     TAssume (print_asm !! (rs !!! "R30") = None);;
+    (* NOTE What are the exact semantics here if I say exists and then assume.
+       Is it the same as assume? - Think about what it means to refine this spec *)
+    args ← TExist _;
+    TAssert (print_args (rs !!! "R0") args);;
+    TVis (Outgoing, EASyscallCall args mem);;
+    '(ret, mem) ← TReceive (λ '(ret, mem), (Incoming, EASyscallRet ret mem));
+    TVis (Outgoing, EAJump (<["PC" := rs !!! "R30"]> $
+                            <["R0" := ret]> $
+                            <["R8" := __NR_PRINT]> $
+                            rs) mem)).
+
+Definition print_spec' : spec asm_event unit void :=
+  Spec.forever (
+    '(rs, mem) ← TReceive (λ '(rs, mem), (Incoming, EAJump rs mem));
+    TAssume (rs !!! "PC" = print_addr);;
+    TAssume (print_asm' !! (rs !!! "R30") = None);;
+    (* NOTE What are the exact semantics here if I say exists and then assume.
+       Is it the same as assume? - Think about what it means to refine this spec *)
     args ← TExist _;
     TAssert (print_args (rs !!! "R0") args);;
     TVis (Outgoing, EASyscallCall args mem);;
@@ -45,15 +72,18 @@ Local Ltac go_i :=
 Lemma print_asm_refines_spec :
   trefines (asm_mod print_asm) (spec_mod print_spec tt).
 Proof.
-  apply: tsim_implies_trefines => n0 /=.
+  apply: tsim_implies_trefines => n0.
+  (* What does this simpl do here? *)
+  simpl.
   unshelve eapply tsim_remember. { simpl. exact (λ _ σa '(t, _),
     t ≡ print_spec ∧
     σa.(asm_cur_instr) = AWaiting ∧
     σa.(asm_instrs) = print_asm). }
   { split!. } { done. }
   move => n _ Hloop [????] [??] ?. destruct!/=.
-  tstep_i => ????? Hi. tstep_s. rewrite -/print_spec. go.
+  tstep_i => ?? rs' ?? Hi. tstep_s. rewrite -/print_spec. go.
   go_s. eexists (_, _). go.
+  (* Set Typeclasses Debug. *)
   go_s. split!. go.
   go_s => ?. go.
   go_s => ?. go.
@@ -76,4 +106,45 @@ Proof.
   by apply: Hloop.
   Unshelve.
   - split; [done|by simplify_map_eq'].
+Qed.
+
+Lemma print_asm_refines_spec' :
+  trefines (asm_mod print_asm') (spec_mod print_spec' tt).
+Proof.
+  apply: tsim_implies_trefines => n0 /=.
+  unshelve eapply tsim_remember. { simpl. exact (λ _ σa '(t, _),
+    t ≡ print_spec' ∧
+    σa.(asm_cur_instr) = AWaiting ∧
+    σa.(asm_instrs) = print_asm'). }
+  { split!. } { done. }
+  move => n _ Hloop [????] [??] ?. destruct!/=.
+  tstep_i => ?? rs' mem' ? Hi. tstep_s. rewrite -/print_spec. go.
+  go_s. eexists (_, _). go.
+  (* Set Typeclasses Debug. *)
+  go_s. split!. go.
+  go_s => ?. go.
+  go_s => ?. go.
+  tstep_i => ??. simplify_map_eq'.
+  tstep_i.
+  tstep_i.
+  tstep_i => ??. simplify_map_eq'.
+  set args := (extract_syscall_args (<["PC":=print_addr + 1 + 1]> (<["R8":=__NR_PRINT]> rs'))).
+  go_s. eexists args. go.
+  go_s. split; [shelve|]. go.
+  (* Noop *)
+  tstep_i. tstep_i. tstep_i => ??. simplify_map_eq'.
+  (* Set Typeclasses Debug. *)
+  tstep_i.
+  go_s. split!.
+  { f_equal. subst args. unfold extract_syscall_args. simpl. rewrite Z.add_0_r. by simplify_map_eq'. }
+  go. tstep_i => ? ?.
+  go_s. eexists (_, _). go.
+  go_s. split!. go.
+  tstep_i. tstep_i => ? ?. simplify_map_eq'.
+  tstep_i. tstep_i => ? ?. sort_map_insert. simplify_map_eq'.
+  go_s. split!;[by sort_map_insert|].
+  go.
+  by apply: Hloop.
+  Unshelve.
+  - subst args. split; [done| by simplify_map_eq'].
 Qed.
